## 9.3
- Known $x=0,x'=-200m$, to find $t$:
$$
    x'=\gamma(x-ut)
$$
或用尺缩
- To find $t'$:
$$
    x=\gamma(x'+ut')
$$
## 9.16
- Conservation of mass-energy:

$$
    m_{n_0}c^2=m_{p_0}c^2+m_ec^2+E_\nu
$$
- Conservation of 动量:

$$
    \begin{aligned}
        p_e+p_\nu &= 0\\
        E_\nu &= cp_\nu\\
        E_e^2 &= p_e^2c^2+E_0^2\\
        \frac{1}{c}\sqrt{E_e^2-E_0^2} &= \frac{E_\nu}{c}\\
    \end{aligned}
$$
## 11.9
$$
    \begin{aligned}
        \eta &= \frac{W}{\Delta Q_{BC}}\\
         &= \frac{\Delta Q_{BC}-\Delta Q_{AD}}{\Delta Q_{BC}}\\
         &=1-\frac{\Delta Q_{AD}}{\Delta Q_{BC}} \\
         &=1-\frac{T_D-T_A}{T_C-T_B} \\
    \end{aligned}
$$

## 12.8
$$
    \Delta S=(\int_{333K}^{T_f}+\int_{T_f}^{288})\frac{mcdT}{T}+\frac{\Delta Q_s}{T_s}
$$

## 12.12
show that 
$$
    \big(\dfrac{\partial \mu}{\partial V_m}\big)_T=V_m \big(\dfrac{\partial p}{\partial V_m}\big)_T
$$

<br>

$$
    \begin{aligned}
        d\mu &=-sdT+vdp \\
        \big(\dfrac{\partial \mu}{\partial v}\big)_T &=\big(\dfrac{\partial \mu}{\partial p}\big)_T \big(\dfrac{\partial p}{\partial v}\big)_T=v \big(\dfrac{\partial p}{\partial v}\big)_T \\
        or:&\\
         d\mu&=-sdT+v[\big(\dfrac{\partial p}{\partial T}\big)_vdT+\big(\dfrac{\partial p}{\partial v}\big)_Tdv] \\
         &= \\
    \end{aligned}
$$

## 12.13 
show that 
$$
    \begin{aligned}
        TdS &= C_pdT-TV\alpha dp\\
        TdS &= C_VdT+T\frac{\alpha}{\kappa}dV\\
    \end{aligned}
$$

<br>


$$
    \begin{aligned}
        dH &= TdS+Vdp\\
         &= T \big(\dfrac{\partial S}{\partial T}\big)_pdT+[T \big(\dfrac{\partial S}{\partial p}\big)_T+V]dp\\
        C_p &= \big(\dfrac{\partial H}{\partial T}\big)_p=T \big(\dfrac{\partial S}{\partial T}\big)_p\\
        \big(\dfrac{\partial H}{\partial p}\big)_T &= T \big(\dfrac{\partial S}{\partial p}\big)_T+V=-T \big(\dfrac{\partial V}{\partial T}\big)_p+V\\
    \end{aligned}
$$
Thus 
$$
    \begin{aligned}
        TdS &= T \big(\dfrac{\partial S}{\partial T}\big)_pdT+T \big(\dfrac{\partial S}{\partial p}\big)_Tdp \\
         &=C_pdT-T \big(\dfrac{\partial V}{\partial T}\big)_pdp \\
         &=C_pdT-TV\alpha dp \\
    \end{aligned}
$$
and 
$$
    \begin{aligned}
        TdS &= T \big(\dfrac{\partial S}{\partial T}\big)_VdT+T \big(\dfrac{\partial S}{\partial V}\big)_TdV\\
         &= C_VdT+T \big(\dfrac{\partial p}{\partial T}\big)_VdV\\
         Cyclic\ chain\ rule&:\\
         &= C_VdT-T \frac{\big(\dfrac{\partial V}{\partial T}\big)_p}{\big(\dfrac{\partial V}{\partial p}\big)_T}dV\\
         &= C_VdT+T\frac{\alpha}{\kappa}dV\\
    \end{aligned}
$$

## 12.11
show that 
$$
    \begin{aligned}
        \big(\dfrac{\partial C_V}{\partial V}\big)_T &=T \big(\dfrac{\partial ^2p}{\partial T^2}\big)_V \\
        \big(\dfrac{\partial C_p}{\partial V}\big)_T &=T \big(\dfrac{\partial ^2V}{\partial T^2}\big)_p \\
    \end{aligned}
$$
<br>

$$
    \begin{aligned}
        \big(\dfrac{\partial C_V}{\partial V}\big)_T &=T \big(\dfrac{\partial \big(\dfrac{\partial S}{\partial T}\big)_V}{\partial V}\big)_T \\
         &=T \big(\dfrac{\partial \big(\dfrac{\partial S}{\partial V}\big)_T}{\partial T}\big)_V \\
        &=T \big(\dfrac{\partial \big(\dfrac{\partial p}{\partial T}\big)_V}{\partial T}\big)_V \\
         &= T \big(\dfrac{\partial ^2p}{\partial T^2}\big)_V\\
    \end{aligned}
$$


show 
$$
    \frac{\kappa_T}{\kappa_S}=\frac{C_p}{C_V}
$$

<br>

$$
    TdS=\big(\dfrac{\partial U}{\partial p}\big)_Vdp+[\big(\dfrac{\partial U}{\partial V}\big)_p+p]dV
$$
Let $dS=0$,we have
$$
    \begin{aligned}
        \big(\dfrac{\partial V}{\partial p}\big)_S &= -\frac{\big(\dfrac{\partial U}{\partial p}\big)_V}{\big(\dfrac{\partial U}{\partial V}\big)_p+p}\\
        \big(\dfrac{\partial U}{\partial p}\big)_V &= \big(\dfrac{\partial U}{\partial T}\big)_V \big(\dfrac{\partial T}{\partial p}\big)_V\\
         &=C_V \big(\dfrac{\partial T}{\partial p}\big)_V \\
        \big(\dfrac{\partial U}{\partial V}\big)_p &=\big(\dfrac{\partial U}{\partial T}\big)_p \big(\dfrac{\partial T}{\partial V}\big)_p \\
        \big(\dfrac{\partial U}{\partial V}\big)_p+p &=\Big[\big(\dfrac{\partial U}{\partial T}\big)_p + p \big(\dfrac{\partial V}{\partial T}\big)_p\Big]\big(\dfrac{\partial T}{\partial V}\big)_p \\
        &=C_p \big(\dfrac{\partial T}{\partial V}\big)_p\\
    \end{aligned}
$$
Therefore, 
$$
    \begin{aligned}
        \big(\dfrac{\partial V}{\partial p}\big)_S &= -\frac{\big(\dfrac{\partial U}{\partial p}\big)_V}{\big(\dfrac{\partial U}{\partial V}\big)_p+p}\\
         &=-\frac{C_V}{C_p} \frac{\big(\dfrac{\partial T}{\partial p}\big)_V}{\big(\dfrac{\partial T}{\partial V}\big)_p} \\
         &=\frac{C_V}{C_p} \big(\dfrac{\partial V}{\partial p}\big)_T\\
    \end{aligned}
$$
移项得证.      